Add an implementation of lists and two implementations of queues

src/linear/adt/Queue2.dfy
@@ -1,25 +1,70 @@
-trait Queue {
+include "../../../src/linear/implementation/SinglyLinkedListWithLast.dfy"
+include "../../../src/linear/interface/Queue.dfy"
+
+class Queue2 extends Queue {
+  var list: SinglyLinkedListWithLast<int>;
+
   function SizeOfRepr(): nat
     ensures SizeOfRepr() > 0
+  {
+    2
+  }
+
+  function Repr0(): set<object>
+    reads this
+  {
+    {list}
+  }
+
+  function Repr1(): set<object>
+    reads this, Repr0()
+  {
+    Repr0() + {list.list}
+  }
+
+  function Repr2(): set<object>
+    reads this, Repr1()
+  {
+    Repr1() + list.Repr()
+  }
 
   function ReprFamily(n: nat): set<object>
     decreases n
     requires n <= SizeOfRepr()
     ensures n > 0 ==> ReprFamily(n) >= ReprFamily(n-1)
     reads this, if n == 0 then {} else ReprFamily(n-1)
-
-  function Repr(): set<object>
-    reads this, ReprFamily(SizeOfRepr()-1)
   {
-    ReprFamily(SizeOfRepr())
+    if n == 0 then
+      Repr0()
+    else if n == 1 then
+      Repr1()
+    else if n == 2 then
+      Repr2()
+    else
+      assert false;
+      {}
   }
 
   predicate Valid()
     reads this, Repr()
+  {
+    list.Valid()
+  }
 
   function Model(): seq<int>
     reads this, Repr()
     requires Valid()
+  {
+    list.Model()
+  }
+
+  constructor()
+    ensures Valid()
+    ensures Model() == []
+    ensures fresh(Repr())
+  {
+    list := new SinglyLinkedListWithLast();
+  }
 
   method Front() returns (x: int)
     requires Valid()
@@ -27,6 +72,9 @@ trait Queue {
     ensures Valid()
     ensures Model() == old(Model())
     ensures x == Model()[0]
+  {
+    x := list.Front();
+  }
 
   method Enqueue(x: int)
     modifies Repr()
@@ -35,6 +83,9 @@ trait Queue {
     ensures Model() == old(Model()) + [x]
     ensures Repr() > old(Repr())
     ensures fresh(Repr() - old(Repr()))
+  {
+    list.PushBack(x);
+  }
 
   method Dequeue() returns (x: int)
     modifies Repr()
@@ -43,4 +94,7 @@ trait Queue {
     ensures Valid()
     ensures [x] + Model() == old(Model())
     ensures Repr() < old(Repr())
+  {
+    x := list.PopFront();
+  }
 }
